Removed effects from context

Refinery/Ctx/Basic.lean
@@ -5,262 +5,261 @@ namespace Refinery
 
 universe u v
 
-structure Var? (α : Type u) (ε : Type v) where
+structure Var? (α : Type u) where
   ty : Ty α
   q : EQuant
-  eff : ε
 
-abbrev Var?.erase (v : Var? α ε) : Var? α ε := ⟨v.ty, 0, v.eff⟩
+abbrev Var?.erase (v : Var? α) : Var? α := ⟨v.ty, 0⟩
 
 @[simp]
-theorem Var?.erase_erase (v : Var? α ε) : v.erase.erase = v.erase := rfl
+theorem Var?.erase_erase (v : Var? α) : v.erase.erase = v.erase := rfl
 
 @[simp]
 abbrev ety_var {α : Type u} (a : Ty α) : EQuant → Ty α
   | 0 => .unit
   | (q : Quant) => a
 
-abbrev Var?.ety {α ε} (v : Var? α ε) : Ty α := ety_var v.ty v.q
+abbrev Var?.ety (v : Var? α) : Ty α := ety_var v.ty v.q
 
-theorem Var?.ety_quant_zero {A : Ty α} {e : ε} : Var?.ety ⟨A, 0, e⟩ = Ty.unit := rfl
+theorem Var?.ety_quant_zero {A : Ty α} : Var?.ety ⟨A, 0⟩ = Ty.unit := rfl
 
-theorem Var?.ety_quant_ty {A : Ty α} {q : Quant} {e : ε} : Var?.ety ⟨A, q, e⟩ = A := rfl
+theorem Var?.ety_quant_ty {A : Ty α} {q : Quant} : Var?.ety ⟨A, q⟩ = A := rfl
 
-theorem Var?.ety_erase {v : Var? α ε} : v.erase.ety = Ty.unit := rfl
+theorem Var?.ety_erase {v : Var? α} : v.erase.ety = Ty.unit := rfl
 
-def Ctx? (α : Type u) (ε : Type v) := List (Var? α ε)
+def Ctx? (α : Type u) := List (Var? α)
 
 variable {α : Type u} {ε : Type v}
 
 @[match_pattern]
-def Ctx?.nil : Ctx? α ε := []
+def Ctx?.nil : Ctx? α := []
 
 @[match_pattern]
-def Ctx?.cons (Γ : Ctx? α ε) (v : Var? α ε) : Ctx? α ε := List.cons v Γ
+def Ctx?.cons (Γ : Ctx? α) (v : Var? α) : Ctx? α := List.cons v Γ
 
-def Ctx?.erase (Γ : Ctx? α ε) : Ctx? α ε := Γ.map Var?.erase
-
-@[simp]
-theorem Ctx?.erase_nil : Ctx?.erase (.nil : Ctx? α ε) = .nil := rfl
+def Ctx?.erase (Γ : Ctx? α) : Ctx? α := Γ.map Var?.erase
 
 @[simp]
-theorem Ctx?.erase_cons (Γ : Ctx? α ε) (v : Var? α ε)
+theorem Ctx?.erase_nil : Ctx?.erase (.nil : Ctx? α) = .nil := rfl
+
+@[simp]
+theorem Ctx?.erase_cons (Γ : Ctx? α) (v : Var? α)
   : Ctx?.erase (Ctx?.cons Γ v) = Ctx?.cons (Ctx?.erase Γ) v.erase := rfl
 
 @[match_pattern]
-abbrev Ctx?.cons' (Γ : Ctx? α ε) (A : Ty α) (q : EQuant) (e : ε) : Ctx? α ε
-  := Γ.cons ⟨A, q, e⟩
+abbrev Ctx?.cons' (Γ : Ctx? α) (A : Ty α) (q : EQuant) : Ctx? α
+  := Γ.cons ⟨A, q⟩
 
 @[elab_as_elim, cases_eliminator]
-def Ctx?.casesOn {motive : Ctx? α ε → Sort _} (Γ : Ctx? α ε)
+def Ctx?.casesOn {motive : Ctx? α → Sort _} (Γ : Ctx? α)
   (nil : motive .nil)
   (cons : ∀ Γ v, motive (.cons Γ v))
   : motive Γ := match Γ with | .nil => nil | .cons Γ v => cons Γ v
 
 @[elab_as_elim, induction_eliminator]
-def Ctx?.inductionOn {motive : Ctx? α ε → Sort _} (Γ : Ctx? α ε)
+def Ctx?.inductionOn {motive : Ctx? α → Sort _} (Γ : Ctx? α)
   (nil : motive .nil)
   (cons : ∀ Γ v, motive Γ → motive (Ctx?.cons Γ v))
   : motive Γ := match Γ with | .nil => nil | .cons Γ v => cons Γ v (inductionOn Γ nil cons)
 
 @[simp]
-theorem Ctx?.erase_erase (Γ : Ctx? α ε) : Ctx?.erase (Ctx?.erase Γ) = Ctx?.erase Γ := by
+theorem Ctx?.erase_erase (Γ : Ctx? α) : Ctx?.erase (Ctx?.erase Γ) = Ctx?.erase Γ := by
   induction Γ <;> simp [*]
 
-def Ctx?.length (Γ : Ctx? α ε) : ℕ := List.length Γ
+def Ctx?.length (Γ : Ctx? α) : ℕ := List.length Γ
 
 @[simp]
-theorem Ctx?.length_nil : Ctx?.length (.nil : Ctx? α ε) = 0 := rfl
+theorem Ctx?.length_nil : Ctx?.length (.nil : Ctx? α) = 0 := rfl
 
 @[simp]
-theorem Ctx?.length_cons (Γ : Ctx? α ε) (v : Var? α ε)
+theorem Ctx?.length_cons (Γ : Ctx? α) (v : Var? α)
   : Ctx?.length (Ctx?.cons Γ v) = Ctx?.length Γ + 1 := rfl
 
-theorem Ctx?.length_cons' (Γ : Ctx? α ε) (A : Ty α) (q : EQuant) (e : ε)
-  : Ctx?.length (Ctx?.cons' Γ A q e) = Ctx?.length Γ + 1 := rfl
+theorem Ctx?.length_cons' (Γ : Ctx? α) (A : Ty α) (q : EQuant)
+  : Ctx?.length (Ctx?.cons' Γ A q) = Ctx?.length Γ + 1 := rfl
 
 @[simp]
-def Ctx?.ety : Ctx? α ε → Ty α
+def Ctx?.ety : Ctx? α → Ty α
   | .nil => Ty.unit
   | .cons Γ v => .tensor (Ctx?.ety Γ) v.ety
 
 @[ext]
-theorem Var?.ext {v w : Var? α ε}
-  (h : v.ty = w.ty) (h' : v.q = w.q) (h'' : v.eff = w.eff) : v = w :=
-  by cases v; cases w; cases h; cases h'; cases h''; rfl
+theorem Var?.ext {v w : Var? α}
+  (h : v.ty = w.ty) (h' : v.q = w.q) : v = w :=
+  by cases v; cases w; cases h; cases h'; rfl
 
-abbrev Var?.unused (v : Var? α ε) : Prop := v.q = 0
+abbrev Var?.unused (v : Var? α) : Prop := v.q = 0
 
 @[simp]
-theorem Var?.unused.eq_erase {v : Var? α ε} (h : v.unused) : v.erase = v
+theorem Var?.unused.eq_erase {v : Var? α} (h : v.unused) : v.erase = v
   := by cases v; cases h; rfl
 
-abbrev Var?.used (v : Var? α ε) : Prop := 1 ≤ v.q
+abbrev Var?.used (v : Var? α) : Prop := 1 ≤ v.q
 
-theorem Var?.used_iff {v : Var? α ε} : v.used ↔ ¬v.unused := EQuant.one_le_iff_ne_zero _
+theorem Var?.used_iff {v : Var? α} : v.used ↔ ¬v.unused := EQuant.one_le_iff_ne_zero _
 
-theorem Var?.unused_iff {v : Var? α ε} : v.unused ↔ ¬v.used := by simp [used_iff]
+theorem Var?.unused_iff {v : Var? α} : v.unused ↔ ¬v.used := by simp [used_iff]
 
 variable [HasQuant α]
 
 open HasQuant
 
-instance Var?.hasQuant : HasQuant (Var? α ε) where
+instance Var?.hasQuant : HasQuant (Var? α) where
   quant v := match v.q with | 0 => ⊤ | (q : Quant) => q ⊓ quant v.ty
 
-instance Ctx?.hasQuant : HasQuant (Ctx? α ε) where
+instance Ctx?.hasQuant : HasQuant (Ctx? α) where
   quant Γ := Γ.foldr (λv q => q ⊓ quant v) ⊤
 
-@[simp] theorem Ctx?.quant_nil : quant (.nil : Ctx? α ε) = ⊤ := rfl
+@[simp] theorem Ctx?.quant_nil : quant (.nil : Ctx? α) = ⊤ := rfl
 
 @[simp]
-theorem Ctx?.quant_cons (Γ : Ctx? α ε) (v : Var? α ε)
+theorem Ctx?.quant_cons (Γ : Ctx? α) (v : Var? α)
   : quant (Ctx?.cons Γ v) = quant Γ ⊓ quant v := rfl
 
 @[simp]
-theorem Var?.quant_erase (v : Var? α ε) : quant (Var?.erase v) = ⊤ := rfl
+theorem Var?.quant_erase (v : Var? α) : quant (Var?.erase v) = ⊤ := rfl
 
 @[simp]
-theorem Ctx?.quant_erase (Γ : Ctx? α ε) : quant (Ctx?.erase Γ) = ⊤ := by induction Γ <;> simp [*]
+theorem Ctx?.quant_erase (Γ : Ctx? α) : quant (Ctx?.erase Γ) = ⊤ := by induction Γ <;> simp [*]
 
-abbrev Var?.del (v : Var? α ε) : Prop := IsAff v
+abbrev Var?.del (v : Var? α) : Prop := IsAff v
 
-abbrev Var?.copy (v : Var? α ε) : Prop := IsRel v
+abbrev Var?.copy (v : Var? α) : Prop := IsRel v
 
-instance Var?.del.instZeroQuant (A : Ty α) (e : ε) : (⟨A, 0, e⟩ : Var? α ε).del
+instance Var?.del.instZeroQuant (A : Ty α) : (⟨A, 0⟩ : Var? α).del
   := ⟨by simp [quant]⟩
 
-instance Var?.copy.instZeroQuant (A : Ty α) (e : ε) : (⟨A, 0, e⟩ : Var? α ε).copy
+instance Var?.copy.instZeroQuant (A : Ty α) : (⟨A, 0⟩ : Var? α).copy
   := ⟨by simp [quant]⟩
 
 @[simp]
-instance Var?.del.instErase (v : Var? α ε) : v.erase.del := ⟨by simp⟩
+instance Var?.del.instErase (v : Var? α) : v.erase.del := ⟨by simp⟩
 
 @[simp]
-instance Var?.copy.instErase (v : Var? α ε) : v.erase.copy := ⟨by simp⟩
+instance Var?.copy.instErase (v : Var? α) : v.erase.copy := ⟨by simp⟩
 
-theorem Var?.del.q (v : Var? α ε) [hv : v.del] : 0 ≤ v.q := by
-  cases v with | mk A q e => cases q using EQuant.casesZero with
+theorem Var?.del.q (v : Var? α) [hv : v.del] : 0 ≤ v.q := by
+  cases v with | mk A q => cases q using EQuant.casesZero with
   | zero => simp
   | rest => simp only [IsAff.is_aff_iff, quant, le_inf_iff] at hv; exact hv.1
 
-theorem Var?.del.ty (v : Var? α ε) [hv : v.del] (h : v.used) : IsAff v.ty := by
-  cases v with | mk A q e => cases q using EQuant.casesZero with
+theorem Var?.del.ty (v : Var? α) [hv : v.del] (h : v.used) : IsAff v.ty := by
+  cases v with | mk A q => cases q using EQuant.casesZero with
   | zero => simp at h
   | rest => simp only [IsAff.is_aff_iff, quant, le_inf_iff] at *; exact hv.2
 
-theorem Var?.del_iff (v : Var? α ε) : v.del ↔ 0 ≤ v.q ∧ (v.used -> IsAff v.ty) := by
-  cases v with | mk A q e => cases q using EQuant.casesZero with
+theorem Var?.del_iff (v : Var? α) : v.del ↔ 0 ≤ v.q ∧ (v.used -> IsAff v.ty) := by
+  cases v with | mk A q => cases q using EQuant.casesZero with
   | zero => simp [quant, IsAff.is_aff_iff]
   | rest q => simp [quant, IsAff.is_aff_iff, quant]; intro _; cases q <;> decide
 
-structure Var?.scopy (v : Var? α ε) : Prop where
+structure Var?.scopy (v : Var? α) : Prop where
   q : EQuant.copy ≤ v.q
   ty : IsRel v.ty
 
-theorem Var?.scopy_iff (v : Var? α ε) : v.scopy ↔ (EQuant.copy ≤ v.q ∧ IsRel v.ty)
+theorem Var?.scopy_iff (v : Var? α) : v.scopy ↔ (EQuant.copy ≤ v.q ∧ IsRel v.ty)
   := ⟨λh => ⟨h.1, h.2⟩, λh => ⟨h.1, h.2⟩⟩
 
-theorem Var?.used.scopy {v : Var? α ε} (h : v.used) [hv : v.copy] : v.scopy := by
-  cases v with | mk A q e => cases q using EQuant.casesZero with
+theorem Var?.used.scopy {v : Var? α} (h : v.used) [hv : v.copy] : v.scopy := by
+  cases v with | mk A q => cases q using EQuant.casesZero with
   | zero => simp at h
   | rest => simp only [IsRel.is_rel_iff, quant, le_inf_iff] at hv; exact ⟨hv.1, ⟨hv.2⟩⟩
 
-theorem Var?.unused.del {v : Var? α ε} (h : v.unused) : v.del
+theorem Var?.unused.del {v : Var? α} (h : v.unused) : v.del
   := by simp only [unused] at h; simp [IsAff.is_aff_iff, quant, h]
 
-theorem Var?.unused.copy {v : Var? α ε} (h : v.unused) : v.copy
+theorem Var?.unused.copy {v : Var? α} (h : v.unused) : v.copy
   := by simp only [unused] at h; simp [IsRel.is_rel_iff, quant, h]
 
 @[simp]
-theorem Var?.unused.quant_top {v : Var? α ε} (h : v.unused) : quant v = ⊤ := by simp [quant, h]
+theorem Var?.unused.quant_top {v : Var? α} (h : v.unused) : quant v = ⊤ := by simp [quant, h]
 
-theorem Var?.scopy.copy {v : Var? α ε} (h : v.scopy) : v.copy := by
-  cases v with | mk A q e => cases q using EQuant.casesZero with
+theorem Var?.scopy.copy {v : Var? α} (h : v.scopy) : v.copy := by
+  cases v with | mk A q => cases q using EQuant.casesZero with
   | zero => simp [IsRel.is_rel_iff, quant]
   | rest => simp [IsRel.is_rel_iff, quant]; constructor; exact h.q; exact h.ty.copy_le_quant
 
-theorem Var?.copy_iff (v : Var? α ε) : v.copy ↔ (v.used -> v.scopy)
+theorem Var?.copy_iff (v : Var? α) : v.copy ↔ (v.used -> v.scopy)
   := ⟨λ_ u => u.scopy, λh => if u : v.unused then u.copy else (h (used_iff.mpr u)).copy⟩
 
-instance Var?.del.instTopQuant (A : Ty α) [IsAff A] (e : ε) : (⟨A, ⊤, e⟩ : Var? α ε).del
+instance Var?.del.instTopQuant (A : Ty α) [IsAff A] : (⟨A, ⊤⟩ : Var? α).del
   := by simp [del_iff, *]
 
-instance Var?.copy.instTopQuant (A : Ty α) [IsRel A] (e : ε) : (⟨A, ⊤, e⟩ : Var? α ε).copy
+instance Var?.copy.instTopQuant (A : Ty α) [IsRel A] : (⟨A, ⊤⟩ : Var? α).copy
   := by simp [copy_iff, scopy_iff, *]
 
-instance Var?.del.instDelQuant (A : Ty α) [IsAff A] (e : ε) : (⟨A, .del, e⟩ : Var? α ε).del
+instance Var?.del.instDelQuant (A : Ty α) [IsAff A] : (⟨A, .del⟩ : Var? α).del
   := by simp [del_iff, *]
 
-instance Var?.copy.instCopyQuant (A : Ty α) [IsRel A] (e : ε) : (⟨A, .copy, e⟩ : Var? α ε).copy
+instance Var?.copy.instCopyQuant (A : Ty α) [IsRel A] : (⟨A, .copy⟩ : Var? α).copy
   := by simp [copy_iff, scopy_iff, *]
 
-theorem Ctx?.quant_le_of_quant_le_cons (Γ : Ctx? α ε) (h : q ≤ quant (Γ.cons v)) : q ≤ quant Γ
+theorem Ctx?.quant_le_of_quant_le_cons (Γ : Ctx? α) (h : q ≤ quant (Γ.cons v)) : q ≤ quant Γ
   := by simp at h; exact h.1
 
-theorem Ctx?.quant_le_var_of_quant_le_cons (Γ : Ctx? α ε) (h : q ≤ quant (Γ.cons v)) : q ≤ quant v
+theorem Ctx?.quant_le_var_of_quant_le_cons (Γ : Ctx? α) (h : q ≤ quant (Γ.cons v)) : q ≤ quant v
   := by simp at h; exact h.2
 
-instance Var?.copy.ety_rel (v : Var? α ε) [h : v.copy] : IsRel v.ety := by
-  cases v with | mk A q e => cases q using EQuant.casesZero with
+instance Var?.copy.ety_rel (v : Var? α) [h : v.copy] : IsRel v.ety := by
+  cases v with | mk A q => cases q using EQuant.casesZero with
   | zero => simp only [ety]; infer_instance
   | rest => simp [quant, IsRel.is_rel_iff] at h; exact ⟨h.2⟩
 
-instance Var?.del.ety_aff (v : Var? α ε) [h : v.del] : IsAff v.ety := by
-  cases v with | mk A q e => cases q using EQuant.casesZero with
+instance Var?.del.ety_aff (v : Var? α) [h : v.del] : IsAff v.ety := by
+  cases v with | mk A q => cases q using EQuant.casesZero with
   | zero => simp only [ety]; infer_instance
   | rest => simp [quant, IsAff.is_aff_iff] at h; exact ⟨h.2⟩
 
-abbrev Ctx?.copy (Γ : Ctx? α ε) : Prop := IsRel Γ
+abbrev Ctx?.copy (Γ : Ctx? α) : Prop := IsRel Γ
 
-abbrev Ctx?.del (Γ : Ctx? α ε) : Prop := IsAff Γ
-
-@[simp]
-instance Ctx?.nil_copy : (.nil : Ctx? α ε).copy := ⟨by simp⟩
+abbrev Ctx?.del (Γ : Ctx? α) : Prop := IsAff Γ
 
 @[simp]
-instance Ctx?.nil_del : (.nil : Ctx? α ε).del := ⟨by simp⟩
+instance Ctx?.nil_copy : (.nil : Ctx? α).copy := ⟨by simp⟩
 
 @[simp]
-instance Ctx?.erase_copy (Γ : Ctx? α ε) : Γ.erase.copy := ⟨by induction Γ <;> simp [*]⟩
+instance Ctx?.nil_del : (.nil : Ctx? α).del := ⟨by simp⟩
 
 @[simp]
-instance Ctx?.erase_del (Γ : Ctx? α ε) : Γ.erase.del := ⟨by induction Γ <;> simp [*]⟩
+instance Ctx?.erase_copy (Γ : Ctx? α) : Γ.erase.copy := ⟨by induction Γ <;> simp [*]⟩
 
 @[simp]
-theorem Ctx?.cons_copy_iff (Γ : Ctx? α ε) (v : Var? α ε) : (Γ.cons v).copy ↔ Γ.copy ∧ v.copy
+instance Ctx?.erase_del (Γ : Ctx? α) : Γ.erase.del := ⟨by induction Γ <;> simp [*]⟩
+
+@[simp]
+theorem Ctx?.cons_copy_iff (Γ : Ctx? α) (v : Var? α) : (Γ.cons v).copy ↔ Γ.copy ∧ v.copy
   := ⟨λ⟨h⟩ => by simp at h; exact ⟨⟨h.1⟩, ⟨h.2⟩⟩, λ⟨⟨hΓ⟩, ⟨hv⟩⟩ => ⟨by simp [*]⟩⟩
 
 @[simp]
-theorem Ctx?.copy.tail (Γ : Ctx? α ε) (v : Var? α ε) [h : (Γ.cons v).copy] : Γ.copy
+theorem Ctx?.copy.tail (Γ : Ctx? α) (v : Var? α) [h : (Γ.cons v).copy] : Γ.copy
   := by rw [cons_copy_iff] at h; exact h.1
 
 @[simp]
-theorem Ctx?.copy.head (Γ : Ctx? α ε) (v : Var? α ε) [h : (Γ.cons v).copy] : v.copy
+theorem Ctx?.copy.head (Γ : Ctx? α) (v : Var? α) [h : (Γ.cons v).copy] : v.copy
   := by rw [cons_copy_iff] at h; exact h.2
 
 @[simp]
-instance Ctx?.copy.cons (Γ : Ctx? α ε) (v : Var? α ε) [Γ.copy] [v.copy] : (Γ.cons v).copy
+instance Ctx?.copy.cons (Γ : Ctx? α) (v : Var? α) [Γ.copy] [v.copy] : (Γ.cons v).copy
   := ⟨by simp [cons_copy_iff, *]⟩
 
 @[simp]
-theorem Ctx?.cons_del_iff (Γ : Ctx? α ε) (v : Var? α ε) : (Γ.cons v).del ↔ Γ.del ∧ v.del
+theorem Ctx?.cons_del_iff (Γ : Ctx? α) (v : Var? α) : (Γ.cons v).del ↔ Γ.del ∧ v.del
   := ⟨λ⟨h⟩ => by simp at h; exact ⟨⟨h.1⟩, ⟨h.2⟩⟩, λ⟨⟨hΓ⟩, ⟨hv⟩⟩ => ⟨by simp [*]⟩⟩
 
 @[simp]
-theorem Ctx?.del.tail (Γ : Ctx? α ε) (v : Var? α ε) [h : (Γ.cons v).del] : Γ.del
+theorem Ctx?.del.tail (Γ : Ctx? α) (v : Var? α) [h : (Γ.cons v).del] : Γ.del
   := by rw [cons_del_iff] at h; exact h.1
 
 @[simp]
-theorem Ctx?.del.head (Γ : Ctx? α ε) (v : Var? α ε) [h : (Γ.cons v).del] : v.del
+theorem Ctx?.del.head (Γ : Ctx? α) (v : Var? α) [h : (Γ.cons v).del] : v.del
   := by rw [cons_del_iff] at h; exact h.2
 
 @[simp]
-instance Ctx?.del.cons (Γ : Ctx? α ε) (v : Var? α ε) [Γ.del] [v.del] : (Γ.cons v).del
+instance Ctx?.del.cons (Γ : Ctx? α) (v : Var? α) [Γ.del] [v.del] : (Γ.cons v).del
   := ⟨by simp [cons_del_iff, *]⟩
 
 @[simp]
-instance Ctx?.ety_rel_of_copy {Γ : Ctx? α ε} [h : Γ.copy] : IsRel (Ctx?.ety Γ) := by
+instance Ctx?.ety_rel_of_copy {Γ : Ctx? α} [h : Γ.copy] : IsRel (Ctx?.ety Γ) := by
   generalize h = h
   induction Γ with
   | nil => constructor; simp [ety]
@@ -271,7 +270,7 @@ instance Ctx?.ety_rel_of_copy {Γ : Ctx? α ε} [h : Γ.copy] : IsRel (Ctx?.ety 
     apply IsRel.tensor
 
 @[simp]
-instance Ctx?.ety_aff_of_del {Γ : Ctx? α ε} [h : Γ.del] : IsAff (Ctx?.ety Γ) := by
+instance Ctx?.ety_aff_of_del {Γ : Ctx? α} [h : Γ.del] : IsAff (Ctx?.ety Γ) := by
   generalize h = h
   induction Γ with
   | nil => constructor; simp [ety]
@@ -281,86 +280,80 @@ instance Ctx?.ety_aff_of_del {Γ : Ctx? α ε} [h : Γ.del] : IsAff (Ctx?.ety Γ
     simp only [ety]
     apply IsAff.tensor
 
-variable [PartialOrder ε]
-
-structure Var?.Wk (v w : Var? α ε) : Prop where
+structure Var?.Wk (v w : Var? α) : Prop where
   ty : v.ty = w.ty
   q : w.q ≤ v.q
-  eff : v.eff ≤ w.eff
   unused_del : w.unused → v.del
 
-theorem Var?.wk_eff (A : Ty α) (q : EQuant) {e e' : ε} (h : e ≤ e') : Var?.Wk ⟨A, q, e⟩ ⟨A, q, e'⟩
-  := ⟨rfl, le_refl _, h, λh => by convert h.del using 0; simp [del_iff]⟩
+instance Var?.instLE : LE (Var? α) := ⟨Wk⟩
 
-instance Var?.instLE : LE (Var? α ε) := ⟨Wk⟩
+theorem Var?.erase_mono {v w : Var? α} (h : v ≤ w) : v.erase ≤ w.erase := by
+  cases v with | mk A q => cases w with | mk A' q' =>
+    exact ⟨h.ty, le_refl _, λ_ => inferInstance⟩
 
-theorem Var?.erase_mono {v w : Var? α ε} (h : v ≤ w) : v.erase ≤ w.erase := by
-  cases v with | mk A q e => cases w with | mk A' q' e' =>
-    exact ⟨h.ty, le_refl _, h.eff, λ_ => inferInstance⟩
+theorem Var?.used.anti {v w : Var? α} (h : v ≤ w) (hw : w.used) : v.used := hw.trans h.q
 
-theorem Var?.used.anti {v w : Var? α ε} (h : v ≤ w) (hw : w.used) : v.used := hw.trans h.q
-
-theorem Var?.unused.mono {v w : Var? α ε} (h : v ≤ w) : (hv : v.unused) → w.unused
+theorem Var?.unused.mono {v w : Var? α} (h : v ≤ w) : (hv : v.unused) → w.unused
   := by simp only [unused_iff, not_imp_not]; exact used.anti h
 
-theorem Var?.del.anti {v w : Var? α ε} (h : v ≤ w) [hw : w.del] : v.del := open Classical in
+theorem Var?.del.anti {v w : Var? α} (h : v ≤ w) [hw : w.del] : v.del := open Classical in
   if hw' : w.used then
     by rw [del_iff] at *; exact ⟨hw.1.trans h.q, λ_ => h.ty ▸ hw.2 hw'⟩
   else
     h.unused_del (unused_iff.mpr hw')
 
-theorem Var?.scopy.anti {v w : Var? α ε} (h : v ≤ w) (hw : w.scopy) : v.scopy where
+theorem Var?.scopy.anti {v w : Var? α} (h : v ≤ w) (hw : w.scopy) : v.scopy where
   q := hw.q.trans h.q
   ty := h.ty ▸ hw.ty
 
-theorem Var?.used.scopy_anti {v w : Var? α ε} (h : v ≤ w) (hw' : w.used) [hw : w.copy] : v.scopy
+theorem Var?.used.scopy_anti {v w : Var? α} (h : v ≤ w) (hw' : w.used) [hw : w.copy] : v.scopy
   := by rw [copy_iff] at *; exact (hw hw').anti h
 
-theorem Var?.copy.anti {v w : Var? α ε} (h : v ≤ w) [hw : IsRel w] (hw' : w.used) : v.copy
+theorem Var?.copy.anti {v w : Var? α} (h : v ≤ w) [hw : IsRel w] (hw' : w.used) : v.copy
   := (hw'.scopy_anti h).copy
 
-theorem Var?.used.quant_anti {v w : Var? α ε} (h : v ≤ w) (hw : w.used) : quant w ≤ quant v := by
-  cases w with | mk A q e =>
+theorem Var?.used.quant_anti {v w : Var? α} (h : v ≤ w) (hw : w.used) : quant w ≤ quant v := by
+  cases w with | mk A q =>
     cases q using EQuant.casesZero with
     | zero => cases hw
     | rest => cases v; cases h.ty; cases h.q using EQuant.le.casesLE <;> simp [quant]
 
-instance Var?.instPartialOrder : PartialOrder (Var? α ε) where
-  le_refl _ := ⟨rfl, le_refl _, le_refl _, λh => h.del⟩
+instance Var?.instPartialOrder : PartialOrder (Var? α) where
+  le_refl _ := ⟨rfl, le_refl _, λh => h.del⟩
   le_trans _ _ _ h h' :=
-    ⟨h.ty.trans h'.ty, h'.q.trans h.q, h.eff.trans h'.eff, λx => (x.del.anti h').anti h⟩
-  le_antisymm _ _ h h' := ext h.ty (le_antisymm h'.q h.q) (le_antisymm h.eff h'.eff)
+    ⟨h.ty.trans h'.ty, h'.q.trans h.q, λx => (x.del.anti h').anti h⟩
+  le_antisymm _ _ h h' := ext h.ty (le_antisymm h'.q h.q)
 
-theorem Var?.Wk.ety_aff_zero {B : Ty α} {e : ε} (h : v ≤ Var?.mk B 0 e)
+theorem Var?.Wk.ety_aff_zero {B : Ty α} (h : v ≤ Var?.mk B 0)
   : IsAff v.ety := del.ety_aff _ (h := del.anti h)
 
-theorem Var?.Wk.ety_eq_quant {B : Ty α} {q : Quant} {e : ε} (h : v ≤ Var?.mk B q e)
+theorem Var?.Wk.ety_eq_quant {B : Ty α} {q : Quant} (h : v ≤ Var?.mk B q)
   : v.ety = B := by
-  cases v with | mk A q' e' => cases q' using EQuant.casesZero with
+  cases v with | mk A q' => cases q' using EQuant.casesZero with
   | zero => cases h.q using EQuant.le.casesLE
   | rest => cases h.ty; rfl
 
-theorem Var?.Wk.ety_eq_used {v w : Var? α ε} (h : v ≤ w) (hw : w.used) : v.ety = w.ety := by
-  cases w with | mk A q e =>
+theorem Var?.Wk.ety_eq_used {v w : Var? α} (h : v ≤ w) (hw : w.used) : v.ety = w.ety := by
+  cases w with | mk A q =>
     cases q using EQuant.casesZero with
     | zero => cases hw
     | rest => rw [ety_eq_quant h]
 
-inductive Ctx?.PWk : Ctx? α ε → Ctx? α ε → Prop where
+inductive Ctx?.PWk : Ctx? α → Ctx? α → Prop where
   | nil : Ctx?.PWk .nil .nil
   | cons {Γ Δ v w} (h : Ctx?.PWk Γ Δ) (hvw : v ≤ w) : Ctx?.PWk (Ctx?.cons Γ v) (Ctx?.cons Δ w)
 
-theorem Ctx?.PWk.head {Γ Δ v w} (h : PWk (α := α) (ε := ε) (.cons Γ v) (.cons Δ w)) : v ≤ w
+theorem Ctx?.PWk.head {Γ Δ v w} (h : PWk (α := α) (.cons Γ v) (.cons Δ w)) : v ≤ w
   := match h with | Ctx?.PWk.cons _ hvw => hvw
 
-theorem Ctx?.PWk.tail {Γ Δ v w} (h : PWk (α := α) (ε := ε) (.cons Γ v) (.cons Δ w)) : PWk Γ Δ
+theorem Ctx?.PWk.tail {Γ Δ v w} (h : PWk (α := α) (.cons Γ v) (.cons Δ w)) : PWk Γ Δ
   := match h with | Ctx?.PWk.cons h _ => h
 
 @[simp]
-theorem Ctx?.PWk.cons_iff {Γ Δ v w} : PWk (α := α) (ε := ε) (.cons Γ v) (.cons Δ w) ↔ PWk Γ Δ ∧ v ≤ w
+theorem Ctx?.PWk.cons_iff {Γ Δ v w} : PWk (α := α) (.cons Γ v) (.cons Δ w) ↔ PWk Γ Δ ∧ v ≤ w
   := ⟨λ h => ⟨Ctx?.PWk.tail h, Ctx?.PWk.head h⟩, λ ⟨h, h'⟩ => Ctx?.PWk.cons h h'⟩
 
-def Ctx?.PWk.inductionOn {Γ Δ} (h : PWk Γ Δ) {motive : (Γ Δ : Ctx? α ε) → PWk Γ Δ → Sort _}
+def Ctx?.PWk.inductionOn {Γ Δ} (h : PWk Γ Δ) {motive : (Γ Δ : Ctx? α) → PWk Γ Δ → Sort _}
   (nil : motive .nil .nil .nil)
   (cons : ∀ {Γ Δ v w} (h : PWk Γ Δ) (hvw : v ≤ w),
     motive Γ Δ h →
@@ -370,39 +363,39 @@ def Ctx?.PWk.inductionOn {Γ Δ} (h : PWk Γ Δ) {motive : (Γ Δ : Ctx? α ε) 
   | .cons _ _, .cons _ _, h => cons h.tail h.head (inductionOn h.tail nil cons)
 
 @[simp]
-theorem Ctx?.PWk.refl (Γ : Ctx? α ε) : PWk Γ Γ := by induction Γ <;> simp [Ctx?.PWk.nil, *]
+theorem Ctx?.PWk.refl (Γ : Ctx? α) : PWk Γ Γ := by induction Γ <;> simp [Ctx?.PWk.nil, *]
 
-theorem Ctx?.PWk.trans {Γ Δ Ξ : Ctx? α ε} (h : PWk Γ Δ) (h' : PWk Δ Ξ) : PWk Γ Ξ := by
+theorem Ctx?.PWk.trans {Γ Δ Ξ : Ctx? α} (h : PWk Γ Δ) (h' : PWk Δ Ξ) : PWk Γ Ξ := by
   induction h generalizing Ξ <;> cases h'
   simp only [refl]
   simp only [cons_iff, true_and, *]
   apply le_trans <;> assumption
 
-theorem Ctx?.PWk.antisymm {Γ Δ : Ctx? α ε} (h : PWk Γ Δ) (h' : PWk Δ Γ) : Γ = Δ := by
+theorem Ctx?.PWk.antisymm {Γ Δ : Ctx? α} (h : PWk Γ Δ) (h' : PWk Δ Γ) : Γ = Δ := by
   induction h with
   | nil => rfl
   | cons h hvw I => cases h' with
   | cons h' hwv => rw [I h', le_antisymm hvw hwv]
 
-theorem Ctx?.PWk.length {Γ Δ : Ctx? α ε} (h : PWk Γ Δ) : Ctx?.length Γ = Ctx?.length Δ
+theorem Ctx?.PWk.length {Γ Δ : Ctx? α} (h : PWk Γ Δ) : Ctx?.length Γ = Ctx?.length Δ
   := by induction h <;> simp [*]
 
-inductive Ctx?.Wk : Ctx? α ε → Ctx? α ε → Type _ where
+inductive Ctx?.Wk : Ctx? α → Ctx? α → Type _ where
   | nil : Ctx?.Wk .nil .nil
   | cons {Γ Δ v w} (h : Ctx?.Wk Γ Δ) (hvw : v ≤ w) : Ctx?.Wk (Ctx?.cons Γ v) (Ctx?.cons Δ w)
   | skip {Γ Δ v} (h : Ctx?.Wk Γ Δ) (hv : v.del) : Ctx?.Wk (Ctx?.cons Γ v) Δ
 
 @[match_pattern]
-abbrev Ctx?.Wk.scons {Γ Δ : Ctx? α ε} (v : Var? α ε) (ρ : Γ.Wk Δ)
+abbrev Ctx?.Wk.scons {Γ Δ : Ctx? α} (v : Var? α) (ρ : Γ.Wk Δ)
   := ρ.cons (le_refl v)
 
-theorem Ctx?.Wk.length {Γ Δ : Ctx? α ε} (h : Wk Γ Δ) : Ctx?.length Δ ≤ Ctx?.length Γ
+theorem Ctx?.Wk.length {Γ Δ : Ctx? α} (h : Wk Γ Δ) : Ctx?.length Δ ≤ Ctx?.length Γ
   := by induction h <;> simp <;> omega
 
-def Ctx?.PWk.toWk {Γ Δ : Ctx? α ε} (h : PWk Γ Δ) : Wk Γ Δ
+def Ctx?.PWk.toWk {Γ Δ : Ctx? α} (h : PWk Γ Δ) : Wk Γ Δ
   := h.inductionOn (motive := λΓ Δ _ => Wk Γ Δ) .nil (λ_ h m => .cons m h)
 
-theorem Ctx?.Wk.toPWk {Γ Δ : Ctx? α ε} (h : Wk Γ Δ) (h' : Γ.length = Δ.length) : Γ.PWk Δ
+theorem Ctx?.Wk.toPWk {Γ Δ : Ctx? α} (h : Wk Γ Δ) (h' : Γ.length = Δ.length) : Γ.PWk Δ
   := by induction h with
   | nil => exact .nil
   | cons h v I => exact .cons (I (by convert h' using 0; simp)) v
@@ -411,12 +404,12 @@ theorem Ctx?.Wk.toPWk {Γ Δ : Ctx? α ε} (h : Wk Γ Δ) (h' : Γ.length = Δ.l
     rw [<-h', length_cons] at hl
     omega
 
-theorem Ctx?.Wk.antisymm {Γ Δ : Ctx? α ε} (h : Wk Γ Δ) (h' : Wk Δ Γ) : Γ = Δ :=
+theorem Ctx?.Wk.antisymm {Γ Δ : Ctx? α} (h : Wk Γ Δ) (h' : Wk Δ Γ) : Γ = Δ :=
   have hl := le_antisymm h'.length h.length
   PWk.antisymm (h.toPWk hl) (h'.toPWk (hl.symm))
 
 -- toPWk is a faithful functor
-theorem Ctx?.Wk.eq_pwk {Γ Δ : Ctx? α ε} (h : Wk Γ Δ) (h' : Γ.length = Δ.length)
+theorem Ctx?.Wk.eq_pwk {Γ Δ : Ctx? α} (h : Wk Γ Δ) (h' : Γ.length = Δ.length)
   : h = (h.toPWk h').toWk := by induction h with
   | nil => rfl
   | cons h v I =>
@@ -429,64 +422,64 @@ theorem Ctx?.Wk.eq_pwk {Γ Δ : Ctx? α ε} (h : Wk Γ Δ) (h' : Γ.length = Δ.
     rw [<-h', length_cons] at hl
     omega
 
-def Ctx?.Wk.refl (Γ : Ctx? α ε) : Wk Γ Γ := (Ctx?.PWk.refl Γ).toWk
+def Ctx?.Wk.refl (Γ : Ctx? α) : Wk Γ Γ := (Ctx?.PWk.refl Γ).toWk
 
-theorem Ctx?.Wk.eq_refl {Γ : Ctx? α ε} (h : Wk Γ Γ) : h = Wk.refl Γ := eq_pwk h rfl
+theorem Ctx?.Wk.eq_refl {Γ : Ctx? α} (h : Wk Γ Γ) : h = Wk.refl Γ := eq_pwk h rfl
 
-def Ctx?.wk0 (Γ : Ctx? α ε) (v : Var? α ε) [hv : v.del] : Wk (Γ.cons v) Γ := (Wk.refl Γ).skip hv
+def Ctx?.wk0 (Γ : Ctx? α) (v : Var? α) [hv : v.del] : Wk (Γ.cons v) Γ := (Wk.refl Γ).skip hv
 
-def Ctx?.Wk.comp {Γ Δ Ξ : Ctx? α ε} : Wk Γ Δ → Wk Δ Ξ → Wk Γ Ξ
+def Ctx?.Wk.comp {Γ Δ Ξ : Ctx? α} : Wk Γ Δ → Wk Δ Ξ → Wk Γ Ξ
   | .nil, .nil => .nil
   | .cons h hv, .cons h' hv' => .cons (h.comp h') (hv.trans hv')
   | .cons h hv, .skip h' hv' => .skip (h.comp h') (Var?.del.anti hv)
   | .skip h hv, h' => .skip (h.comp h') hv
 
-theorem Ctx?.Wk.comp_assoc {Γ Δ Ξ Θ : Ctx? α ε} (h : Wk Γ Δ) (h' : Wk Δ Ξ) (h'' : Wk Ξ Θ)
+theorem Ctx?.Wk.comp_assoc {Γ Δ Ξ Θ : Ctx? α} (h : Wk Γ Δ) (h' : Wk Δ Ξ) (h'' : Wk Ξ Θ)
   : h.comp (h'.comp h'') = (h.comp h').comp h'' := by induction h generalizing Ξ Θ with
   | nil => cases h'; cases h''; rfl
   | cons _ _ I => cases h' <;> cases h'' <;> simp [comp, I]
   | skip _ _ I => simp [comp, I]
 
 @[simp]
-def Ctx?.Wk.ix {Γ Δ : Ctx? α ε} : Wk Γ Δ → ℕ → ℕ
+def Ctx?.Wk.ix {Γ Δ : Ctx? α} : Wk Γ Δ → ℕ → ℕ
   | .nil => id
   | .cons h _ => Nat.liftWk h.ix
   | .skip h _ => Nat.stepWk h.ix
 
-instance Ctx?.Wk.coeFunRen {Γ Δ : Ctx? α ε} : CoeFun (Wk Γ Δ) (λ_ => ℕ → ℕ) := ⟨ix⟩
+instance Ctx?.Wk.coeFunRen {Γ Δ : Ctx? α} : CoeFun (Wk Γ Δ) (λ_ => ℕ → ℕ) := ⟨ix⟩
 
 @[simp]
-theorem Ctx?.Wk.ix_increasing {Γ Δ : Ctx? α ε} (h : Wk Γ Δ) (i : ℕ) : i ≤ h i := by
+theorem Ctx?.Wk.ix_increasing {Γ Δ : Ctx? α} (h : Wk Γ Δ) (i : ℕ) : i ≤ h i := by
   induction h generalizing i with
   | nil => simp [ix]
   | cons _ _ I => cases i <;> simp [ix, *]
   | skip _ _ I => simp [ix]; have I := I i; omega
 
 @[simp]
-theorem Ctx?.Wk.ix_comp_applied {Γ Δ Ξ : Ctx? α ε} (h : Wk Γ Δ) (h' : Wk Δ Ξ) (i : ℕ)
+theorem Ctx?.Wk.ix_comp_applied {Γ Δ Ξ : Ctx? α} (h : Wk Γ Δ) (h' : Wk Δ Ξ) (i : ℕ)
   : (h.comp h') i = h (h' i) := by induction h generalizing Ξ i with
   | nil => cases h'; rfl
   | cons _ _ I => cases h' <;> cases i <;> simp [comp, ix, I]
   | skip _ _ I => simp [comp, ix, I]
 
-theorem Ctx?.Wk.ix_comp {Γ Δ Ξ : Ctx? α ε} (h : Wk Γ Δ) (h' : Wk Δ Ξ)
+theorem Ctx?.Wk.ix_comp {Γ Δ Ξ : Ctx? α} (h : Wk Γ Δ) (h' : Wk Δ Ξ)
   : (h.comp h').ix = h.ix ∘ h'.ix := funext (λi => Wk.ix_comp_applied h h' i)
 
-theorem Ctx?.Wk.ix_length_eq_applied {Γ Δ : Ctx? α ε}
+theorem Ctx?.Wk.ix_length_eq_applied {Γ Δ : Ctx? α}
   (h : Γ.Wk Δ) (hl : Γ.length = Δ.length) (i : ℕ) : h i = i := by induction h generalizing i with
   | nil => rfl
   | cons _ _ I =>
     cases i; rfl; simp only [ix, Nat.liftWk_succ, add_left_inj]; apply I; convert hl using 0; simp
   | skip h _ => have hl' := h.length; rw [<-hl] at hl'; simp at hl'
 
-theorem Ctx?.Wk.ix_length_eq {Γ Δ : Ctx? α ε} (h : Γ.Wk Δ) (hl : Γ.length = Δ.length)
+theorem Ctx?.Wk.ix_length_eq {Γ Δ : Ctx? α} (h : Γ.Wk Δ) (hl : Γ.length = Δ.length)
   : h.ix = id := funext (λi => ix_length_eq_applied h hl i)
 
-theorem Ctx?.Wk.ix_refl {Γ : Ctx? α ε} (h : Γ.Wk Γ) : h.ix = id := ix_length_eq _ rfl
+theorem Ctx?.Wk.ix_refl {Γ : Ctx? α} (h : Γ.Wk Γ) : h.ix = id := ix_length_eq _ rfl
 
 -- TODO: ix is an injection...
 
-theorem Ctx?.Wk.ix_bounded {Γ Δ : Ctx? α ε} (h : Γ.Wk Δ) (i : ℕ)
+theorem Ctx?.Wk.ix_bounded {Γ Δ : Ctx? α} (h : Γ.Wk Δ) (i : ℕ)
   (hi : i < Δ.length) : h.ix i < Γ.length
   := by induction h generalizing i with
   | nil => simp at hi
@@ -497,30 +490,30 @@ theorem Ctx?.Wk.ix_bounded {Γ Δ : Ctx? α ε} (h : Γ.Wk Δ) (i : ℕ)
       apply I; convert hi using 0; simp
   | skip _ _ I => simp [ix, *]
 
-def Ctx?.Wk.skips {Γ Δ : Ctx? α ε} (h : Wk Γ Δ) : ℕ := h 0
+def Ctx?.Wk.skips {Γ Δ : Ctx? α} (h : Wk Γ Δ) : ℕ := h 0
 
 --TODO: minimize and report because this is a _sin_
-def Ctx?.drop (Γ : Ctx? α ε) [h : Γ.del] : Wk Γ .nil := (λh => match Γ with
+def Ctx?.drop (Γ : Ctx? α) [h : Γ.del] : Wk Γ .nil := (λh => match Γ with
   | .nil => .nil
   | .cons Γ _ => have _ := h.tail; .skip Γ.drop h.head) h
 
 @[simp]
-theorem Ctx?.Wk.drop_nil : (.nil : Ctx? α ε).drop = .nil := rfl
+theorem Ctx?.Wk.drop_nil : (.nil : Ctx? α).drop = .nil := rfl
 
 @[simp]
-theorem Ctx?.Wk.drop_cons (Γ : Ctx? α ε) [hΓ : Γ.del] (v : Var? α ε) [hv : v.del]
+theorem Ctx?.Wk.drop_cons (Γ : Ctx? α) [hΓ : Γ.del] (v : Var? α) [hv : v.del]
   : (Ctx?.cons Γ v).drop = Γ.drop.skip inferInstance := rfl
 
-theorem Ctx?.Wk.drop_del {Γ : Ctx? α ε} (w : Γ.Wk .nil) : Γ.del := by
+theorem Ctx?.Wk.drop_del {Γ : Ctx? α} (w : Γ.Wk .nil) : Γ.del := by
   induction Γ <;> cases w <;> simp; constructor <;> apply_assumption; assumption
 
-theorem Ctx?.wk_nil_eq_drop {Γ : Ctx? α ε} (w : Γ.Wk .nil) : w = Γ.drop (h := w.drop_del) := by
+theorem Ctx?.wk_nil_eq_drop {Γ : Ctx? α} (w : Γ.Wk .nil) : w = Γ.drop (h := w.drop_del) := by
   induction Γ <;> cases w <;> rw [drop]; simp; apply_assumption
 
-theorem Ctx?.wk_nil_unique {Γ : Ctx? α ε} (w w' : Γ.Wk .nil) : w = w' := by
+theorem Ctx?.wk_nil_unique {Γ : Ctx? α} (w w' : Γ.Wk .nil) : w = w' := by
   rw [wk_nil_eq_drop w, wk_nil_eq_drop w']
 
-theorem Ctx?.del.wk {Γ Δ : Ctx? α ε} (h : Γ.Wk Δ) [hΔ : Δ.del] : Γ.del := (λhΔ => by
+theorem Ctx?.del.wk {Γ Δ : Ctx? α} (h : Γ.Wk Δ) [hΔ : Δ.del] : Γ.del := (λhΔ => by
   induction h with
   | nil => infer_instance
   | cons Γ hvw I =>
@@ -533,28 +526,28 @@ theorem Ctx?.del.wk {Γ Δ : Ctx? α ε} (h : Γ.Wk Δ) [hΔ : Δ.del] : Γ.del 
     infer_instance
   ) hΔ
 
-def Ctx?.choose_drop (Γ : Ctx? α ε) (h : Nonempty (Γ.Wk .nil)) : Γ.Wk .nil :=
+def Ctx?.choose_drop (Γ : Ctx? α) (h : Nonempty (Γ.Wk .nil)) : Γ.Wk .nil :=
   have _ : Γ.del := let ⟨h⟩ := h; h.drop_del; Γ.drop
 
-def Var?.Ix (Γ : Ctx? α ε) (v : Var? α ε) : Type _ := Γ.Wk [v]
+def Var?.Ix (Γ : Ctx? α) (v : Var? α) : Type _ := Γ.Wk [v]
 
 @[match_pattern]
-def Var?.zero_le {Γ : Ctx? α ε} (x : Γ.Wk .nil) {v w : Var? α ε} (h : v ≤ w) : Ix (Γ.cons v) w
+def Var?.zero_le {Γ : Ctx? α} (x : Γ.Wk .nil) {v w : Var? α} (h : v ≤ w) : Ix (Γ.cons v) w
   := x.cons h
 
 @[match_pattern]
-abbrev Var?.zero {Γ : Ctx? α ε} (x : Γ.Wk .nil) (v : Var? α ε) : Ix (Γ.cons v) v
+abbrev Var?.zero {Γ : Ctx? α} (x : Γ.Wk .nil) (v : Var? α) : Ix (Γ.cons v) v
   := zero_le x (le_refl v)
 
 @[match_pattern]
-def Var?.Ix.succ {Γ : Ctx? α ε} (v : Var? α ε) [h : v.del] {w} (x : Ix Γ w) : Ix (Γ.cons v) w
+def Var?.Ix.succ {Γ : Ctx? α} (v : Var? α) [h : v.del] {w} (x : Ix Γ w) : Ix (Γ.cons v) w
   := x.skip h
 
 @[elab_as_elim, cases_eliminator]
 def Var?.Ix.casesOn {motive : ∀ {Γ v}, Ix Γ v → Sort _}
   {Γ v} (x : Ix Γ v)
-  (zero_le : ∀ {Γ : Ctx? α ε} (d : Γ.Wk .nil) {v w} (hv : v ≤ w), motive (zero_le d hv))
-  (succ : ∀ {Γ} (v : Var? α ε) (_ : v.del) {w} (x : Ix Γ w), motive (succ v x))
+  (zero_le : ∀ {Γ : Ctx? α} (d : Γ.Wk .nil) {v w} (hv : v ≤ w), motive (zero_le d hv))
+  (succ : ∀ {Γ} (v : Var? α) (_ : v.del) {w} (x : Ix Γ w), motive (succ v x))
   : motive x := match x with
   | .cons d hv => zero_le d hv
   | .skip x hv => succ _ _ x
@@ -562,83 +555,83 @@ def Var?.Ix.casesOn {motive : ∀ {Γ v}, Ix Γ v → Sort _}
 @[elab_as_elim, induction_eliminator]
 def Var?.Ix.inductionOn {motive : ∀ {Γ v}, Ix Γ v → Sort _}
   {Γ v} (x : Ix Γ v)
-  (zero_le : ∀ {Γ : Ctx? α ε} (d : Γ.Wk .nil) {v w} (hv : v ≤ w), motive (zero_le d hv))
-  (succ : ∀ {Γ} {v : Var? α ε} (h : v.del) {w} (x : Ix Γ w), motive x → motive (succ v (h := h) x))
+  (zero_le : ∀ {Γ : Ctx? α} (d : Γ.Wk .nil) {v w} (hv : v ≤ w), motive (zero_le d hv))
+  (succ : ∀ {Γ} {v : Var? α} (h : v.del) {w} (x : Ix Γ w), motive x → motive (succ v (h := h) x))
   : motive x := match x with
   | .cons d hv => zero_le d hv
   | .skip x hv => succ hv x (inductionOn x zero_le succ)
 
-def Var?.Ix.ix {Γ : Ctx? α ε} {v} (x : Ix Γ v) : ℕ := x.skips
+def Var?.Ix.ix {Γ : Ctx? α} {v} (x : Ix Γ v) : ℕ := x.skips
 
 @[simp]
-theorem Var?.ix_zero_le {Γ : Ctx? α ε} {v w : Var? α ε} (h : v ≤ w) (x : Γ.Wk .nil)
+theorem Var?.ix_zero_le {Γ : Ctx? α} {v w : Var? α} (h : v ≤ w) (x : Γ.Wk .nil)
   : (zero_le x h).ix = 0 := rfl
 
 @[simp]
-theorem Var?.Ix.ix_succ {Γ : Ctx? α ε} (v : Var? α ε) [h : v.del] {w} (x : Ix Γ w)
+theorem Var?.Ix.ix_succ {Γ : Ctx? α} (v : Var? α) [h : v.del] {w} (x : Ix Γ w)
   : (succ v x).ix = x.ix + 1 := rfl
 
-def Var?.Ix.wk {Γ Δ : Ctx? α ε} (h : Γ.Wk Δ) {v} (x : Ix Δ v) : Ix Γ v := h.comp x
+def Var?.Ix.wk {Γ Δ : Ctx? α} (h : Γ.Wk Δ) {v} (x : Ix Δ v) : Ix Γ v := h.comp x
 
-theorem Var?.Ix.wk_wk {Γ Δ Ξ : Ctx? α ε} (h : Γ.Wk Δ) (h' : Δ.Wk Ξ) {v} (x : Ix Ξ v)
+theorem Var?.Ix.wk_wk {Γ Δ Ξ : Ctx? α} (h : Γ.Wk Δ) (h' : Δ.Wk Ξ) {v} (x : Ix Ξ v)
   : (x.wk h').wk h = x.wk (h.comp h') := Ctx?.Wk.comp_assoc h h' x
 
-theorem Var?.Ix.wk_comp {Γ Δ Ξ : Ctx? α ε} (h : Γ.Wk Δ) (h' : Δ.Wk Ξ) {v} (x : Ix Ξ v)
+theorem Var?.Ix.wk_comp {Γ Δ Ξ : Ctx? α} (h : Γ.Wk Δ) (h' : Δ.Wk Ξ) {v} (x : Ix Ξ v)
   : x.wk (h.comp h') = (x.wk h').wk h := (x.wk_wk h h').symm
 
 @[simp]
-theorem Var?.Ix.succ_wk_cons {Γ Δ : Ctx? α ε} (h : Γ.Wk Δ)
-  {v v' : Var? α ε} (hv : v ≤ v') [hv' : IsAff v'] {w} (x : Ix Δ w)
+theorem Var?.Ix.succ_wk_cons {Γ Δ : Ctx? α} (h : Γ.Wk Δ)
+  {v v' : Var? α} (hv : v ≤ v') [hv' : IsAff v'] {w} (x : Ix Δ w)
   : (succ _ x).wk (h.cons hv) = (succ _ (h := del.anti hv) (x.wk h)) := rfl
 
 @[simp]
-theorem Var?.Ix.wk_skip {Γ Δ : Ctx? α ε} (h : Γ.Wk Δ)
-  (v : Var? α ε) [hv : IsAff v] {w} (x : Ix Δ w)
+theorem Var?.Ix.wk_skip {Γ Δ : Ctx? α} (h : Γ.Wk Δ)
+  (v : Var? α) [hv : IsAff v] {w} (x : Ix Δ w)
   : x.wk (h.skip hv) = (x.wk h).succ v := rfl
 
 @[simp]
-theorem Var?.Ix.ix_wk {Γ Δ : Ctx? α ε} (h : Γ.Wk Δ) {v} (x : Ix Δ v) : (x.wk h).ix = h.ix x.ix
+theorem Var?.Ix.ix_wk {Γ Δ : Ctx? α} (h : Γ.Wk Δ) {v} (x : Ix Δ v) : (x.wk h).ix = h.ix x.ix
   := by rw [ix, Ctx?.Wk.skips, wk, Ctx?.Wk.ix_comp]; rfl
 
-theorem Var?.Ix.ix_wk_le {Γ Δ : Ctx? α ε} (h : Γ.Wk Δ) {v} (x : Ix Δ v) : x.ix ≤ (x.wk h).ix
+theorem Var?.Ix.ix_wk_le {Γ Δ : Ctx? α} (h : Γ.Wk Δ) {v} (x : Ix Δ v) : x.ix ≤ (x.wk h).ix
   := by simp
 
 -- TODO: ix is an injection on variables...
 
-inductive Ctx?.At (v : Var? α ε) : Ctx? α ε → ℕ → Prop where
+inductive Ctx?.At (v : Var? α) : Ctx? α → ℕ → Prop where
   | here {Γ} (d : Ctx?.Wk Γ .nil) {w} : w ≤ v → Ctx?.At v (Ctx?.cons Γ w) 0
   | there {Γ w n} (x : Ctx?.At v Γ n) (hw : w.del) : Ctx?.At v (Ctx?.cons Γ w) (n + 1)
 
-theorem Ctx?.At.zero_cons_head {Γ : Ctx? α ε} {v} (h : (Γ.cons w).At v 0) : w ≤ v
+theorem Ctx?.At.zero_cons_head {Γ : Ctx? α} {v} (h : (Γ.cons w).At v 0) : w ≤ v
   := by cases h; assumption
 
-def Ctx?.At.zero_cons_tail {Γ : Ctx? α ε} {v} (h : (Γ.cons w).At v 0) : Γ.Wk .nil
+def Ctx?.At.zero_cons_tail {Γ : Ctx? α} {v} (h : (Γ.cons w).At v 0) : Γ.Wk .nil
   := Γ.choose_drop (by cases h; constructor; assumption)
 
-theorem Ctx?.At.succ_cons_head {Γ : Ctx? α ε} {v w} (h : (Γ.cons w).At v (n + 1)) : w.del
+theorem Ctx?.At.succ_cons_head {Γ : Ctx? α} {v w} (h : (Γ.cons w).At v (n + 1)) : w.del
   := by cases h; assumption
 
-theorem Ctx?.At.succ_cons_tail {Γ : Ctx? α ε} {v w} (h : (Γ.cons w).At v (n + 1)) : Γ.At v n
+theorem Ctx?.At.succ_cons_tail {Γ : Ctx? α} {v w} (h : (Γ.cons w).At v (n + 1)) : Γ.At v n
   := by cases h; assumption
 
-theorem Ctx?.At.succ_cons_iff (Γ : Ctx? α ε) (v w) : (Γ.cons w).At v (n + 1) ↔ w.del ∧ Γ.At v n
+theorem Ctx?.At.succ_cons_iff (Γ : Ctx? α) (v w) : (Γ.cons w).At v (n + 1) ↔ w.del ∧ Γ.At v n
   := ⟨λh => ⟨h.succ_cons_head, h.succ_cons_tail⟩, λ⟨h, h'⟩ => At.there h' h⟩
 
 @[elab_as_elim, induction_eliminator]
-def Ctx?.At.inductionOn {v : Var? α ε} {motive : ∀ (Γ n), Ctx?.At v Γ n → Sort _}
+def Ctx?.At.inductionOn {v : Var? α} {motive : ∀ (Γ n), Ctx?.At v Γ n → Sort _}
   (h : Ctx?.At v Γ n)
-  (here : ∀ (Γ : Ctx? α ε) (d : Γ.Wk .nil) (w) (hw : w ≤ v), motive (Γ.cons w) 0 (here d hw))
-  (there : ∀ (Γ) (w : Var? α ε) (n) (x : Ctx?.At v Γ n) (hw : w.del),
+  (here : ∀ (Γ : Ctx? α) (d : Γ.Wk .nil) (w) (hw : w ≤ v), motive (Γ.cons w) 0 (here d hw))
+  (there : ∀ (Γ) (w : Var? α) (n) (x : Ctx?.At v Γ n) (hw : w.del),
     motive Γ n x → motive (Γ.cons w) (n + 1) (there x hw))
   : motive Γ n h := match Γ, n, h with
   | .cons Γ w, 0, h => here Γ h.zero_cons_tail w h.zero_cons_head
   | .cons Γ w, n + 1, h
     => there Γ w n h.succ_cons_tail h.succ_cons_head (h.succ_cons_tail.inductionOn here there)
 
-theorem Ctx?.At.wkOut {v : Var? α ε} {Γ : Ctx? α ε} {n} (h : Γ.At v n) (h' : v ≤ w)
+theorem Ctx?.At.wkOut {v : Var? α} {Γ : Ctx? α} {n} (h : Γ.At v n) (h' : v ≤ w)
   : Γ.At w n := by induction h <;> constructor <;> (try apply le_trans) <;> assumption
 
-theorem Ctx?.At.wkIn {Γ Δ : Ctx? α ε} (w : Γ.Wk Δ) {v : Var? α ε} {n} (h : Δ.At v n)
+theorem Ctx?.At.wkIn {Γ Δ : Ctx? α} (w : Γ.Wk Δ) {v : Var? α} {n} (h : Δ.At v n)
   : Γ.At v (w n) := by induction w generalizing n with
   | nil => cases h
   | skip w hv I => constructor <;> apply_assumption; assumption
@@ -646,14 +639,14 @@ theorem Ctx?.At.wkIn {Γ Δ : Ctx? α ε} (w : Γ.Wk Δ) {v : Var? α ε} {n} (h
   | here => constructor; (apply Wk.comp <;> assumption); (apply le_trans <;> assumption)
   | there => constructor; (apply I; assumption); (exact Var?.del.anti hv)
 
-def Ctx?.At.ix {Γ : Ctx? α ε} {v n} (h : Γ.At v n) : v.Ix Γ
+def Ctx?.At.ix {Γ : Ctx? α} {v n} (h : Γ.At v n) : v.Ix Γ
   := h.inductionOn (λ_ d _ h => Var?.zero_le d h) (λ_ _ _ _ _ I => I.succ _)
 
 @[simp]
-theorem Ctx?.At.ix_ix {Γ : Ctx? α ε} {v n} (h : Γ.At v n) : h.ix.ix = n
+theorem Ctx?.At.ix_ix {Γ : Ctx? α} {v n} (h : Γ.At v n) : h.ix.ix = n
   := by induction h <;> simp [ix, inductionOn]; assumption
 
-theorem Var?.Ix.at {Γ : Ctx? α ε} {v} (x : Ix Γ v) : Γ.At v x.ix
+theorem Var?.Ix.at {Γ : Ctx? α} {v} (x : Ix Γ v) : Γ.At v x.ix
   := by induction x <;> constructor <;> assumption
 
 -- TODO: so therefore at_ix is just the identity
