Refinery/Ctx/Split.lean
@@ -2,14 +2,14 @@ import Refinery.Ctx.Basic
 
 namespace Refinery
 
-variable [HasQuant α] [PartialOrder ε]
+variable [HasQuant α]
 
-inductive Var?.Split : Var? α ε → Var? α ε → Var? α ε → Type _
-  | left {v w} (h : v ≤ w) (e) : Split v w ⟨v.ty, 0, e⟩
-  | right {v w} (h : v ≤ w) (e) : Split v ⟨v.ty, 0, e⟩ w
+inductive Var?.Split : Var? α → Var? α → Var? α → Type _
+  | left {v w} (h : v ≤ w) : Split v w v.erase
+  | right {v w} (h : v ≤ w) : Split v v.erase w
   | sboth {u v w} : u.scopy → u ≤ v → u ≤ w → Split u v w
 
-inductive Ctx?.Split : Ctx? α ε → Ctx? α ε → Ctx? α ε → Type _ where
+inductive Ctx?.Split : Ctx? α → Ctx? α → Ctx? α → Type _ where
   | nil : Ctx?.Split .nil .nil .nil
   | cons {Γ Δ Ξ v l r} (h : Split Γ Δ Ξ) (hvw : v.Split l r)
     : Split (Ctx?.cons Γ v) (Ctx?.cons Δ l) (Ctx?.cons Ξ r)
